separating and converting between cps and cpsk

src/Cps.v
@@ -1,4 +1,4 @@
-Require Import CoqCompile.Lambda CoqCompile.Env.
+Require Import CoqCompile.Lambda CoqCompile.Env CoqCompile.CpsCommon.
 Require Import ExtLib.Data.Strings.
 Require Import ZArith String List Bool.
 Require Import ExtLib.Structures.Monads.
@@ -13,7 +13,6 @@ Require Import ExtLib.Core.ZDecidables.
 Require Import ExtLib.Core.PosDecidables.
 Require Import ExtLib.Tactics.Consider.
 
-
 Set Implicit Arguments.
 Set Strict Implicit.
 
@@ -25,40 +24,6 @@ Module CPS.
   Local Open Scope monad_scope.
   Definition constructor := Lambda.constructor.
   Definition env_t := Lambda.env_t.
-
-  (** Operands are "small" values (fit into a register) and include variables, 
-      zero-arity constructors (e.g., true, false, nil) and integers. *)
-  Inductive op : Type := 
-  | Var_o : var -> op
-  | Con_o : constructor -> op
-  | Int_o : Z -> op.
-
-  (** We compile pattern matching into simple C-like switch expressions, where
-      you can only match an operand against a tag, which is either an integer
-      or symbolic constructor tag. *)
-  Inductive pattern : Type := 
-  | Int_p : Z -> pattern
-  | Con_p : constructor -> pattern.
-
-  (** We have a bunch of primitive operations on values *)
-  Inductive primop : Type := 
-  (* comparisons/tests *) 
-  | Eq_p     (* operand equality *)
-  | Neq_p    (* operand inequality *)
-  | Lt_p     (* integer less than *)
-  | Lte_p    (* integer ltess than or equal *)
-  | Ptr_p    (* is the value a pointer?  used to distinguish nullary constructors *)
-  (* arithmetic *)
-  | Plus_p   (* we don't include division as it's partial *)
-  | Minus_p 
-  | Times_p
-  (* build tuple and projection from a tuple *)
-  | MkTuple_p (* mkTuple_p [v1;...;vn] builds a record of n words and initializes it 
-                 with the values v1,...,vn. *)
-  | Proj_p.   (* Proj_p [Int_o i;v] projects the ith component of the tuple referenced
-                 by v, using zero-based indexing. *)
-
-  Inductive mop : Type := .
 
   (** CPS are in general a sequence of let-bindings that either terminate with 
       a function application, or else fork using a switch into a tree of nested
@@ -81,53 +46,6 @@ Module CPS.
   | Fn_d : var -> list var -> exp -> decl
   | Bind_d : var -> var -> mop -> list op -> decl.
 
-  Global Instance RelDec_primop_eq : RelDec (@eq primop) := 
-  { rel_dec := fun x y =>
-    match x , y with
-      | Eq_p , Eq_p 
-      | Neq_p , Neq_p
-      | Lt_p , Lt_p
-      | Lte_p , Lte_p
-      | Ptr_p , Ptr_p
-      | Plus_p , Plus_p
-      | Minus_p , Minus_p
-      | Times_p , Times_p
-      | MkTuple_p , MkTuple_p 
-      | Proj_p , Proj_p => true
-      | _ , _ => false
-    end }.
-
-  Global Instance RelDecCorrect_primop_eq : RelDec_Correct RelDec_primop_eq.
-  Proof.
-    constructor; destruct x; destruct y; simpl rel_dec; split; intros; subst; try congruence.
-  Qed.
-
-  Global Instance RelDec_mop_eq : RelDec (@eq mop) :=
-  { rel_dec l r := match l , r with
-                   end }.
-
-  Global Instance RelDecCorrect_mop_eq : RelDec_Correct RelDec_mop_eq.
-  Proof.
-    constructor. destruct x.
-  Qed.
-
-  Global Instance RelDec_op_eq : RelDec (@eq op) :=
-  { rel_dec l r := match l , r with
-                     | Var_o l , Var_o r => eq_dec l r
-                     | Con_o l , Con_o r => eq_dec l r
-                     | Int_o l , Int_o r => eq_dec l r
-                     | _ , _ => false
-                   end }.
-
-  Global Instance RelDecCorrect_op_eq : RelDec_Correct RelDec_op_eq.
-  Proof.
-    Opaque Env.RelDec_var_eq RelDec_zeq.
-    constructor. destruct x; destruct y; simpl; unfold eq_dec; try congruence; 
-    try rewrite rel_dec_correct; intuition try congruence.
-    consider (string_dec c c0); intuition congruence.
-    consider (string_dec c c0); intuition congruence.
-    Transparent Env.RelDec_var_eq RelDec_zeq.
-  Qed.
 
   (** Simplify a switch that only has one branch. *)
   Definition switch_e (v:op) (arms: list (pattern * exp)) (def:option exp) := 
@@ -159,36 +77,6 @@ Module CPS.
           | Z0 => "0"%char
           | Zpos p => show p
           | Zneg p => "-"%char << show p
-        end }.
-    Global Instance Show_mop : Show mop :=
-      { show m := match m with end }.
-    
-    Global Instance Show_op : Show op :=
-      { show o :=
-        match o with 
-          | Var_o x => show x
-          | Con_o c => "Con(" << show c << ")"
-          | Int_o i => show i
-        end }.
-    Global Instance Show_pat : Show pattern :=
-      { show p :=
-        match p with 
-          | Int_p i => show i
-          | Con_p c => show c
-        end }.
-    Global Instance Show_primop : Show primop :=
-      { show p := 
-        match p with 
-          | Eq_p => "eq?"
-          | Neq_p => "neq?"
-          | Lt_p => "lt?"
-          | Lte_p => "lte?"
-          | Ptr_p => "ptr?"
-          | Plus_p => "+"
-          | Minus_p => "-"
-          | Times_p => "*"
-          | Proj_p => "#"
-          | MkTuple_p => "mkTuple"
         end }.
 
     Require Import ExtLib.Data.Char.
@@ -235,3 +123,4 @@ Module CPS.
 End CPS.
 
 Export Env.
+Export CpsCommon.
