src/CpsK.v
@@ -1,4 +1,4 @@
-Require Import CoqCompile.Lambda CoqCompile.Env.
+Require Import CoqCompile.Lambda CoqCompile.Env CoqCompile.CpsCommon.
 Require Import ExtLib.Data.Strings.
 Require Import ZArith String List Bool.
 Require Import ExtLib.Structures.Monads.
@@ -32,53 +32,19 @@ Set Strict Implicit.
 (** Defines CPS language datatype, pretty printer, and conversion from Lambda.exp
     to the CPS language.
 *)
-Module CPS.
+Module CPSK.
   Import MonadNotation. 
   Local Open Scope monad_scope.
   Definition constructor := Lambda.constructor.
   Definition env_t := Lambda.env_t.
 
-  (** Operands are "small" values (fit into a register) and include variables, 
-      zero-arity constructors (e.g., true, false, nil) and integers. *)
-  Inductive op : Type := 
-  | Var_o : var -> op
-  | Con_o : constructor -> op
-  | Int_o : Z -> op.
-
-  (** We compile pattern matching into simple C-like switch expressions, where
-      you can only match an operand against a tag, which is either an integer
-      or symbolic constructor tag. *)
-  Inductive pattern : Type := 
-  | Int_p : Z -> pattern
-  | Con_p : constructor -> pattern.
-
-  (** We have a bunch of primitive operations on values *)
-  Inductive primop : Type := 
-  (* comparisons/tests *) 
-  | Eq_p     (* operand equality *)
-  | Neq_p    (* operand inequality *)
-  | Lt_p     (* integer less than *)
-  | Lte_p    (* integer ltess than or equal *)
-  | Ptr_p    (* is the value a pointer?  used to distinguish nullary constructors *)
-  (* arithmetic *)
-  | Plus_p   (* we don't include division as it's partial *)
-  | Minus_p 
-  | Times_p
-  (* build tuple and projection from a tuple *)
-  | MkTuple_p (* mkTuple_p [v1;...;vn] builds a record of n words and initializes it 
-                 with the values v1,...,vn. *)
-  | Proj_p.   (* Proj_p [Int_o i;v] projects the ith component of the tuple referenced
-                 by v, using zero-based indexing. *)
-
   Inductive cont : Type := K : string -> positive -> cont.
-
-  Inductive mop : Type := .
 
   (** CPS are in general a sequence of let-bindings that either terminate with 
       a function application, or else fork using a switch into a tree of nested
       CPS expressions.  *)
   Inductive exp : Type := 
-  | App_e : op -> cont -> list op -> exp
+  | App_e : op -> list cont -> list op -> exp
   | Let_e : decl -> exp -> exp
   | Letrec_e : list decl -> exp -> exp
     (** Switch is only used on small integer values and unlike Match, doesn't do any
@@ -95,38 +61,8 @@ Module CPS.
     (** let x := p(v1,...,vn) *)
   | Prim_d : var -> primop -> list op -> decl
     (** let f := fun (x1,...,xn) => e *)
-  | Fn_d : var -> cont -> list var -> exp -> decl
+  | Fn_d : var -> list cont -> list var -> exp -> decl
   | Bind_d : var -> var -> mop -> list op -> decl.
-
-  Global Instance RelDec_primop_eq : RelDec (@eq primop) := 
-  { rel_dec := fun x y =>
-    match x , y with
-      | Eq_p , Eq_p 
-      | Neq_p , Neq_p
-      | Lt_p , Lt_p
-      | Lte_p , Lte_p
-      | Ptr_p , Ptr_p
-      | Plus_p , Plus_p
-      | Minus_p , Minus_p
-      | Times_p , Times_p
-      | MkTuple_p , MkTuple_p 
-      | Proj_p , Proj_p => true
-      | _ , _ => false
-    end }.
-
-  Global Instance RelDecCorrect_primop_eq : RelDec_Correct RelDec_primop_eq.
-  Proof.
-    constructor; destruct x; destruct y; simpl rel_dec; split; intros; subst; try congruence.
-  Qed.
-
-  Global Instance RelDec_mop_eq : RelDec (@eq mop) :=
-  { rel_dec l r := match l , r with
-                   end }.
-
-  Global Instance RelDecCorrect_mop_eq : RelDec_Correct RelDec_mop_eq.
-  Proof.
-    constructor. destruct x.
-  Qed.
 
   Global Instance RelDec_cont_eq : RelDec (@eq cont) :=
   { rel_dec l r := match l , r with
@@ -139,24 +75,6 @@ Module CPS.
     change (p =? p0)%positive with (rel_dec (equ := eq) p p0).
     consider (string_dec s s0 && rel_dec (equ := eq) p p0); intuition; subst; auto;
     inversion H; auto.
-  Qed.
-
-  Global Instance RelDec_op_eq : RelDec (@eq op) :=
-  { rel_dec l r := match l , r with
-                     | Var_o l , Var_o r => eq_dec l r
-                     | Con_o l , Con_o r => eq_dec l r
-                     | Int_o l , Int_o r => eq_dec l r
-                     | _ , _ => false
-                   end }.
-
-  Global Instance RelDecCorrect_op_eq : RelDec_Correct RelDec_op_eq.
-  Proof.
-    Opaque Env.RelDec_var_eq RelDec_zeq.
-    constructor. destruct x; destruct y; simpl; unfold eq_dec; try congruence; 
-    try rewrite rel_dec_correct; intuition try congruence.
-    consider (string_dec c c0); intuition congruence.
-    consider (string_dec c c0); intuition congruence.
-    Transparent Env.RelDec_var_eq RelDec_zeq.
   Qed.
 
   (** Simplify a switch that only has one branch. *)
@@ -190,36 +108,6 @@ Module CPS.
           | Zpos p => show p
           | Zneg p => "-"%char << show p
         end }.
-    Global Instance Show_mop : Show mop :=
-      { show m := match m with end }.
-    
-    Global Instance Show_op : Show op :=
-      { show o :=
-        match o with 
-          | Var_o x => show x
-          | Con_o c => "Con(" << show c << ")"
-          | Int_o i => show i
-        end }.
-    Global Instance Show_pat : Show pattern :=
-      { show p :=
-        match p with 
-          | Int_p i => show i
-          | Con_p c => show c
-        end }.
-    Global Instance Show_primop : Show primop :=
-      { show p := 
-        match p with 
-          | Eq_p => "eq?"
-          | Neq_p => "neq?"
-          | Lt_p => "lt?"
-          | Lte_p => "lte?"
-          | Ptr_p => "ptr?"
-          | Plus_p => "+"
-          | Minus_p => "-"
-          | Times_p => "*"
-          | Proj_p => "#"
-          | MkTuple_p => "mkTuple"
-        end }.
 
     Global Instance Show_cont : Show cont :=
       { show c :=
@@ -239,7 +127,7 @@ Module CPS.
           in
           "letK " << indent "and  " (sepBy chr_newline (map emitKd ks)) << chr_newline
           << "in " << emitexp e
-        | App_e v k vs => show v << "(" << show k << "; " << sepBy ", " (map show vs) << ")"
+        | App_e v ks vs => show v << "(" << sepBy "," (map show ks) << "; " << sepBy ", " (map show vs) << ")"
         | Let_e d e =>
           "let " << indent "  " (emitdecl d) << " in " << indent "  " (emitexp e)
         | Letrec_e ds e => 
@@ -264,7 +152,7 @@ Module CPS.
         | Prim_d x p vs => 
           show x << " = " << show p << "(" << sepBy " " (map show vs) << ")"
         | Fn_d f k xs e => 
-          show f << "(" << show k << "; " << sepBy (", " : showM) (map show xs) << ") = " << indent "  " (emitexp e)
+          show f << "(" << sepBy "," (map show k) << "; " << sepBy (", " : showM) (map show xs) << ") = " << indent "  " (emitexp e)
         | Bind_d x w mop args =>
           show x << "[" << show w << "] <- " << show mop << "(" << sepBy " " (map show args) << ")"
       end.
@@ -275,7 +163,7 @@ Module CPS.
     Definition exp2string (e:exp) : string := to_string e.
     
   End Printing.
-
-End CPS.
+End CPSK.
 
 Export Env.
+Export CpsCommon.
