src/Cps2CpsK.v
@@ -1,0 +1,32 @@
+Require Import CoqCompile.Cps CoqCompile.CpsK.
+Require Import ExtLib.Structures.Reducible.
+Require Import ExtLib.Data.Option.
+Require Import ExtLib.Data.Lists.
+
+(** There are several translations from Cps to CpsK.
+ ** The simplest just uses nil as all the continuations
+ **)
+
+Fixpoint cps2cpsk_exp (e : CPS.exp) : CPSK.exp :=
+  match e with
+    | CPS.App_e o os =>
+      CPSK.App_e o nil os
+    | CPS.Let_e d e => 
+      CPSK.Let_e (cps2cpsk_decl d) (cps2cpsk_exp e)
+    | CPS.Letrec_e ds e =>
+      CPSK.Letrec_e (map cps2cpsk_decl ds) (cps2cpsk_exp e)
+    | CPS.Switch_e o ps d =>
+      let ps := map (fun p_e => let '(p,e) := p_e in
+        (p, cps2cpsk_exp e)) ps in
+      let d := map cps2cpsk_exp d in
+      CPSK.Switch_e o ps d        
+    | CPS.Halt_e o o' =>
+      CPSK.Halt_e o o'
+  end
+with cps2cpsk_decl (d : CPS.decl) : CPSK.decl :=
+  match d with
+    | CPS.Op_d v o => CPSK.Op_d v o
+    | CPS.Prim_d v p os => CPSK.Prim_d v p os
+    | CPS.Bind_d v w p os => CPSK.Bind_d v w p os
+    | CPS.Fn_d v args body => CPSK.Fn_d v nil args (cps2cpsk_exp body)      
+  end.
