src/CpsCommon.v
@@ -1,0 +1,135 @@
+Require Import CoqCompile.Env CoqCompile.Lambda.
+Require Import BinNums.
+
+Set Implicit Arguments.
+Set Strict Implicit.
+
+(** Operands are "small" values (fit into a register) and include variables, 
+    zero-arity constructors (e.g., true, false, nil) and integers. *)
+Inductive op : Type := 
+| Var_o : var -> op
+| Con_o : Lambda.constructor -> op
+| Int_o : Z -> op.
+
+(** We compile pattern matching into simple C-like switch expressions, where
+   you can only match an operand against a tag, which is either an integer
+   or symbolic constructor tag. *)
+Inductive pattern : Type := 
+| Int_p : Z -> pattern
+| Con_p : Lambda.constructor -> pattern.
+
+(** We have a bunch of primitive operations on values *)
+Inductive primop : Type := 
+(* comparisons/tests *) 
+| Eq_p     (* operand equality *)
+| Neq_p    (* operand inequality *)
+| Lt_p     (* integer less than *)
+| Lte_p    (* integer ltess than or equal *)
+| Ptr_p    (* is the value a pointer?  used to distinguish nullary constructors *)
+(* arithmetic *)
+| Plus_p   (* we don't include division as it's partial *)
+| Minus_p 
+| Times_p
+(* build tuple and projection from a tuple *)
+| MkTuple_p (* mkTuple_p [v1;...;vn] builds a record of n words and initializes it 
+               with the values v1,...,vn. *)
+| Proj_p.   (* Proj_p [Int_o i;v] projects the ith component of the tuple referenced
+               by v, using zero-based indexing. *)
+
+(** Monadic operations **)
+Inductive mop : Type := .
+
+Section decidables.
+  Require Import ExtLib.Core.RelDec.
+  Require Import ExtLib.Core.ZDecidables.
+  Require Import ExtLib.Core.PosDecidables.
+  Require Import ExtLib.Data.Strings.
+  Require Import ExtLib.Tactics.Consider.
+
+  Global Instance RelDec_primop_eq : RelDec (@eq primop) := 
+  { rel_dec := fun x y =>
+    match x , y with
+      | Eq_p , Eq_p 
+      | Neq_p , Neq_p
+      | Lt_p , Lt_p
+      | Lte_p , Lte_p
+      | Ptr_p , Ptr_p
+      | Plus_p , Plus_p
+      | Minus_p , Minus_p
+      | Times_p , Times_p
+      | MkTuple_p , MkTuple_p 
+      | Proj_p , Proj_p => true
+      | _ , _ => false
+    end }.
+
+  Global Instance RelDecCorrect_primop_eq : RelDec_Correct RelDec_primop_eq.
+  Proof.
+    constructor; destruct x; destruct y; simpl rel_dec; split; intros; subst; try congruence.
+  Qed.
+
+  Global Instance RelDec_mop_eq : RelDec (@eq mop) :=
+  { rel_dec l r := match l , r with
+                   end }.
+
+  Global Instance RelDecCorrect_mop_eq : RelDec_Correct RelDec_mop_eq.
+  Proof.
+    constructor. destruct x.
+  Qed.
+
+  Global Instance RelDec_op_eq : RelDec (@eq op) :=
+  { rel_dec l r := match l , r with
+                     | Var_o l , Var_o r => eq_dec l r
+                     | Con_o l , Con_o r => eq_dec l r
+                     | Int_o l , Int_o r => eq_dec l r
+                     | _ , _ => false
+                   end }.
+
+  Global Instance RelDecCorrect_op_eq : RelDec_Correct RelDec_op_eq.
+  Proof.
+    Opaque Env.RelDec_var_eq RelDec_zeq.
+    constructor. destruct x; destruct y; simpl; unfold eq_dec; try congruence; 
+    try rewrite rel_dec_correct; intuition try congruence.
+    consider (string_dec c c0); intuition congruence.
+    consider (string_dec c c0); intuition congruence.
+    Transparent Env.RelDec_var_eq RelDec_zeq.
+  Qed.
+End decidables.
+
+Section Printing.
+  Require Import ExtLib.Programming.Show.
+  Require Import Ascii.
+  Import ShowNotation.
+  Local Open Scope string_scope.
+  Local Open Scope show_scope.
+
+  Global Instance Show_mop : Show mop :=
+  { show m := match m with end }.
+    
+  Global Instance Show_op : Show op :=
+  { show o :=
+    match o with 
+      | Var_o x => show x
+      | Con_o c => "Con(" << show c << ")"
+      | Int_o i => show i
+    end }.
+  Global Instance Show_pat : Show pattern :=
+  { show p :=
+    match p with 
+      | Int_p i => show i
+      | Con_p c => show c
+    end }.
+  Global Instance Show_primop : Show primop :=
+  { show p := 
+    match p with 
+      | Eq_p => "eq?"
+      | Neq_p => "neq?"
+      | Lt_p => "lt?"
+      | Lte_p => "lte?"
+      | Ptr_p => "ptr?"
+      | Plus_p => "+"
+      | Minus_p => "-"
+      | Times_p => "*"
+      | Proj_p => "#"
+      | MkTuple_p => "mkTuple"
+    end }.
+End Printing.
