src/CpsK2Cps.v
@@ -1,0 +1,46 @@
+Require Import CoqCompile.Cps CoqCompile.CpsK.
+Require Import ExtLib.Structures.Reducible.
+Require Import ExtLib.Data.Option.
+Require Import ExtLib.Data.Lists.
+
+(** Converting from CpsK to Cps requires that we convert
+ ** all of the second-class continuations into first-class
+ ** functions
+ **)
+
+Definition cont2var (c : CPSK.cont) : Env.var :=
+  match c with
+    | CPSK.K n p => Env.mkVar (Some n) p
+  end.
+
+Fixpoint cpsk2cps_exp (e : CPSK.exp) : CPS.exp :=
+  match e with
+    | CPSK.App_e o ks os =>
+      CPS.App_e o ((map (fun x => CpsCommon.Var_o (cont2var x)) ks) ++ os)
+    | CPSK.Let_e d e => 
+      CPS.Let_e (cpsk2cps_decl d) (cpsk2cps_exp e)
+    | CPSK.Letrec_e ds e =>
+      CPS.Letrec_e (map cpsk2cps_decl ds) (cpsk2cps_exp e)
+    | CPSK.Switch_e o ps d =>
+      let ps := map (fun p_e => let '(p,e) := p_e in
+        (p, cpsk2cps_exp e)) ps in
+      let d := map cpsk2cps_exp d in
+      CPS.Switch_e o ps d        
+    | CPSK.Halt_e o o' =>
+      CPS.Halt_e o o'
+
+    | CPSK.AppK_e k os =>
+      CPS.App_e (CpsCommon.Var_o (cont2var k)) os
+    | CPSK.LetK_e ks e =>
+      CPS.Letrec_e 
+      (map (fun k_args_body => let '(k,args,body) := k_args_body in
+              CPS.Fn_d (cont2var k) args (cpsk2cps_exp body)) ks)
+      (cpsk2cps_exp e)
+  end
+with cpsk2cps_decl (d : CPSK.decl) : CPS.decl :=
+  match d with
+    | CPSK.Op_d v o => CPS.Op_d v o
+    | CPSK.Prim_d v p os => CPS.Prim_d v p os
+    | CPSK.Bind_d v w p os => CPS.Bind_d v w p os
+    | CPSK.Fn_d v ks args body => CPS.Fn_d v args (cpsk2cps_exp body)      
+  end.
