src/Optimize.v
@@ -1,24 +1,27 @@
-Require Import CoqCompile.Cps.
 Require Import List.
 
 Set Implicit Arguments.
 Set Strict Implicit.
 
 Module Optimize.
-  Import CPS.
 
-  Definition optimization : Type := exp -> exp.
+  Section parametric.
+    Variable exp : Type.
 
-  Fixpoint optSeq (os : list optimization) : optimization :=
-    match os with
-      | nil => fun x => x
-      | o :: os => fun x => optSeq os (o x)
-    end.
 
-  Fixpoint optRepeat (n : nat) (o : optimization) : optimization :=
-    match n with
-      | 0 => o
-      | S n => fun x => optRepeat n o (o x)
-    end.
+    Definition optimization : Type := exp -> exp.
+    
+    Fixpoint optSeq (os : list optimization) : optimization :=
+      match os with
+        | nil => fun x => x
+        | o :: os => fun x => optSeq os (o x)
+      end.
+    
+    Fixpoint optRepeat (n : nat) (o : optimization) : optimization :=
+      match n with
+        | 0 => o
+        | S n => fun x => optRepeat n o (o x)
+      end.
+  End parametric.
 
 End Optimize.
